src/coq_formalism/reduce.v
@@ -17,19 +17,19 @@ Section Reducer.
 
     Context {measurement : Type}.
     Context {corruption : Type}.
-    (* Context {G : attackgraph measurement corruption}.*)
+    Context {G : attackgraph measurement corruption}.
 
     (* Labels and States must have decidable equality *)
     Hypothesis eqDec_measurement : forall (x y : measurement), {x = y} + {x <> y}.
     Hypothesis eqDec_corruption : forall (x y : corruption), {x = y} + {x <> y}.
-    Hypothesis eqDec_state :  forall (G : attackgraph measurement corruption) (x y : G.(state _ _)), {x = y} + {x <> y}.
+    Hypothesis eqDec_state :  forall (x y : G.(state _ _)), {x = y} + {x <> y}.
 
     (* steps are equivalent or not equivalent *)
-    Lemma eqDec_step : forall (G : attackgraph measurement corruption) (x y : (G.(state _ _) * G.(state _ _))), {x = y} + {x <> y}.
+    Lemma eqDec_step : forall (x y : (G.(state _ _) * G.(state _ _))), {x = y} + {x <> y}.
     Proof.
-        intros G x y;
+        intros x y;
         destruct x as [stx stx']; destruct y as [sty sty'].
-        destruct eqDec_state with (G := G) (x:=stx) (y:=sty).
+        destruct eqDec_state with (x:=stx) (y:=sty).
         + destruct eqDec_state with (x:=stx') (y:=sty').
         ++ subst. left. eauto.  
         ++ right. intros contra. rewrite pair_equal_spec in contra. destruct contra. contradiction.
@@ -39,31 +39,31 @@ Section Reducer.
     Qed.
 
     (* list of steps are decidably equal *)
-    Lemma eqDec_list_steps: forall `{G : attackgraph measurement corruption} (x y : list (G.(state _ _) * G.(state _ _))), {x = y} + {x <> y}.
+    Lemma eqDec_list_steps: forall (x y : list (G.(state _ _) * G.(state _ _))), {x = y} + {x <> y}.
     Proof.
-        intros G. apply list_eq_dec. apply eqDec_step.
+        intros G0. apply list_eq_dec. apply eqDec_step.
     Qed.
 
-    Fixpoint replace_measurement_incomplete {G: attackgraph measurement corruption} (Steps : list (G.(state _ _) * G.(state _ _))) (st st' : (G.(state _ _))) : 
+    Fixpoint replace_measurement_incomplete (Steps : list (G.(state _ _) * G.(state _ _))) (st st' : (G.(state _ _))) : 
                                  list (G.(state _ _) * G.(state _ _)) := 
         match Steps with 
-        | (st1, st2) :: Steps' => if (eqDec_state G st st2)
+        | (st1, st2) :: Steps' => if (eqDec_state st st2)
                                   then (st1, st') :: replace_measurement_incomplete Steps' st st' 
                                   else (st1, st2) :: replace_measurement_incomplete Steps' st st'
         | nil => Steps 
         end. 
 
     (* Replace all occurences of st by st' in Steps *)
-    Fixpoint replace_measurement {G : attackgraph measurement corruption} (Steps : list (G.(state _ _) * G.(state _ _))) 
+    Fixpoint replace_measurement (Steps : list (G.(state _ _) * G.(state _ _))) 
     (st st' : G.(state _ _)) : 
     list (G.(state _ _) * G.(state _ _)) :=
     match Steps with
     | (st1, st2) :: Steps' => 
-        if (eqDec_state G st1 st)
-        then if (eqDec_state G st2 st)
+        if (eqDec_state st1 st)
+        then if (eqDec_state st2 st)
             then (st', st') :: replace_measurement Steps' st st'
             else (st', st2) :: replace_measurement Steps' st st'
-        else if (eqDec_state G st2 st)
+        else if (eqDec_state st2 st)
             then (st1, st') :: replace_measurement Steps' st st'
             else (st1, st2) :: replace_measurement Steps' st st'
     | nil => Steps
@@ -72,13 +72,13 @@ Section Reducer.
     Print eqDec_step.
     Print remove.
 
-    Fixpoint find_measurement {G : attackgraph measurement corruption} (AllSteps Steps : list (G.(state _ _) * G.(state _ _))) :  list (G.(state _ _) * G.(state _ _)) := 
+    Fixpoint find_measurement (AllSteps Steps : list (G.(state _ _) * G.(state _ _))) :  list (G.(state _ _) * G.(state _ _)) := 
     match Steps with 
     | (st, st') :: Steps' => match (G.(label _ _) st) with 
                              | inr c1 => find_measurement AllSteps Steps' 
                              | inl m1 => match (G.(label _ _) st') with 
                                          (* if both m1 and m2 are measurement events then you can replace them *)
-                                         | inl m2 => replace_measurement (remove (eqDec_step _ ) (st, st') AllSteps) st st' 
+                                         | inl m2 => replace_measurement (remove (eqDec_step ) (st, st') AllSteps) st st' 
                                          | _ => find_measurement AllSteps Steps'
                                          end
                              end
@@ -86,7 +86,7 @@ Section Reducer.
     end.
 
     (* finding measurement x in x should return x? *)
-    Lemma find_measurement_helper : forall (G : attackgraph measurement corruption) (x : list(G.(state _ _) * G.(state _ _))), find_measurement x x = x.
+    Lemma find_measurement_helper : forall (x : list(G.(state _ _) * G.(state _ _))), find_measurement x x = x.
     Proof.
         intros. induction x.
         + auto.
@@ -96,7 +96,7 @@ Section Reducer.
         ++++ simpl. unfold remove. unfold replace_measurement.*)
     Abort.
 
-    Definition reduce1 `{G : attackgraph measurement corruption} (Steps : list (G.(state _ _) * G.(state _ _))) : list (G.(state _ _) * G.(state _ _)) :=
+    Definition reduce1 (Steps : list (G.(state _ _) * G.(state _ _))) : list (G.(state _ _) * G.(state _ _)) :=
     find_measurement Steps Steps.
 
     (* We cannot define a recursive fixpoint because of 
@@ -108,13 +108,13 @@ Section Reducer.
      * then the graph cannot be further reduced. If reduce1
      * does not return itself, then the reduction call is
      * recursed. *)
-    Inductive reducer {G : attackgraph measurement corruption} : list (G.(state _ _) * G.(state _ _)) -> list (G.(state _ _) * G.(state _ _)) -> Prop :=
+    Inductive reducer : list (G.(state _ _) * G.(state _ _)) -> list (G.(state _ _) * G.(state _ _)) -> Prop :=
     | reduce_done : forall x, reduce1 x = x -> reducer x x
     | reduce_more : forall x y, reduce1 x <> x -> reducer (reduce1 x) y -> reducer x y.  
 
     Definition step_update (g1 : attackgraph measurement corruption) (newSteps : list (g1.(state _ _) * g1.(state _ _))) :=  {| state := g1.(state _ _) ; steps := newSteps ; label := g1.(label _ _) |}. 
 
-    Theorem  reducer_deterministic : forall G1 (x y z : list (G1.(state _ _) * G1.(state _ _))), 
+    Theorem  reducer_deterministic : forall (x y z : list (G.(state _ _) * G.(state _ _))), 
         reducer x y -> reducer x z -> y = z.
     Proof.
         intros.
@@ -128,9 +128,9 @@ Section Reducer.
     Qed.
     
     (* if a graph reduces from x to y and then y to z then you can say x reduces to z *)
-    Theorem  reducer_trans : forall (G : attackgraph measurement corruption) (x : list(G.(state _ _) * G.(state _ _))) (y : list(G.(state _ _) * G.(state _ _))) , reducer x y -> forall (z : list(G.(state _ _) * G.(state _ _))) , reducer y z -> reducer x z.
+    Theorem  reducer_trans : forall (x : list(G.(state _ _) * G.(state _ _))) (y : list(G.(state _ _) * G.(state _ _))) , reducer x y -> forall (z : list(G.(state _ _) * G.(state _ _))) , reducer y z -> reducer x z.
     Proof.
-        intros G x y Hxy. induction Hxy.
+        intros x y Hxy. induction Hxy.
         + eauto.
         + intros. apply reduce_more; eauto.
     Qed.
