src/coq_formalism/compare.v
@@ -1,0 +1,39 @@
+(************************
+ * comparison over sets of
+ * attack graphs 
+ *************************)
+
+Require Import Coq.Lists.List.
+
+Require Import Order.attack_graph.
+Require Import Order.strict_partial_order.
+Require Import Order.reduce.
+Require Import Order.equiv.
+Require Import Order.utilities.
+Require Import Order.partial_order.
+Require Import Order.supports.
+
+Section Compare.
+
+  Context {measurement : Type}.
+  Context {corruption : Type}. 
+
+  (* 4 mutually exclusive ordering relations 
+   * less than or equal to 
+   * greater than or equal to 
+   * equal 
+   * incomparable *)
+
+  Inductive ord := 
+  | lte 
+  | gte 
+  | eq
+  | incomp. 
+
+  Inductive compare (g1 g2 : list (attackgraph measurement corruption)) : ord -> Prop :=
+  | lte' : supports g1 g2 -> compare g1 g2 lte
+  | gte' : supports g2 g1 -> compare g1 g2 gte
+  | eq' : set_eq g1 g2 -> compare g1 g2 eq
+  | incomp' : ~ supports g1 g2 -> ~ supports g2 g1 -> ~ set_eq g1 g2 -> compare g1 g2 incomp.
+
+End Compare.
